clock_independnce_WIP

pancake/semantics/proofs/panItreeSemEquivScript.sml
@@ -195,7 +195,7 @@ Proof
   drule itreeTauTheory.itree_bind_resp_t_wbisim >>
   rw [itree_bind_left_ident_wbisim]
 QED
-
+(*
 (* TODO: Finish this *)
 Theorem msem_ret_wbisim_eq:
   mrec_sem ht ≈ Ret x ⇒
@@ -377,16 +377,44 @@ Theorem fbs_sem_clock_inv_thm:
 Proof
   cheat
 QED
-
+*)
 
 (* Main correspondence theorem *)
 
 (* Extension for ffi$behaviour capturing evaluation result
  of convergent computations *)
 Datatype:
+  bstate =
+    <| locals      : varname |-> 'a v
+     ; code        : funname |-> ((varname # shape) list # ('a panLang$prog))
+                     (* arguments (with shape), body *)
+     ; eshapes     : eid |-> shape
+     ; memory      : 'a word -> 'a word_lab
+     ; memaddrs    : ('a word) set
+     ; sh_memaddrs    : ('a word) set
+     ; be          : bool
+     ; ffi         : 'ffi ffi_state
+     ; base_addr   : 'a word |>
+End
+
+Definition unclock_def:
+  unclock (s:('a,'b) panSem$state) =
+    <| locals      := s.locals
+     ; code        := s.code
+     ; eshapes     := s.eshapes
+     ; memory      := s.memory
+     ; memaddrs    := s.memaddrs
+     ; sh_memaddrs := s.sh_memaddrs
+     ; be          := s.be
+     ; ffi         := s.ffi
+     ; base_addr   := s.base_addr
+|>
+End  
+
+Datatype:
   sem_behaviour =
     SemDiverge (io_event llist)
-    | SemTerminate (('a result option) # ('a,'b) state) (io_event list)
+    | SemTerminate (('a result option) # ('a,'b) bstate) (io_event list)
     | SemFail
 End
 
@@ -394,7 +422,8 @@ Definition fbs_semantics_beh_def:
   fbs_semantics_beh s prog =
   if ∃k. FST $ panSem$evaluate (prog,s with clock := k) ≠ SOME TimeOut
   then (case some (r,s'). ∃k. evaluate (prog,s with clock := k) = (r,s') ∧ r ≠ SOME TimeOut of
-         SOME (r,s') => (case r of
+         SOME (r,s') => let s' = unclock s' in
+                        (case r of
                            SOME (Return _) => SemTerminate (r,s') s'.ffi.io_events
                          | SOME (FinalFFI _) => SemTerminate (r,s') s'.ffi.io_events
                          | SOME Error => SemFail
@@ -409,7 +438,7 @@ Definition itree_semantics_beh_def:
   itree_semantics_beh s prog =
   let lt = ltree_lift query_oracle s.ffi (mrec_sem (h_prog (prog,s))) in
       case some (r,s'). lt ≈ Ret (r,s') of
-      | SOME (r,s') => let s' = s' with clock := 0 in
+      | SOME (r,s') => let s' = unclock s' in
                          (case r of
                       SOME TimeOut => SemTerminate (r,s') s'.ffi.io_events
                     | SOME (FinalFFI _) => SemTerminate (r,s') s'.ffi.io_events
@@ -521,7 +550,7 @@ Proof
 QED
 
 Theorem fbs_semantics_beh_simps:
-  (∃k. fbs_semantics_beh s Skip = SemTerminate (NONE,s with clock := k) s.ffi.io_events) ∧
+  (∃k. fbs_semantics_beh s Skip = SemTerminate (NONE,unclock s) s.ffi.io_events) ∧
   (eval s e = NONE ⇒ fbs_semantics_beh s (Dec v e prog) ≠ SemTerminate p l)
 Proof
   rw []
@@ -529,13 +558,12 @@ Proof
           panSemTheory.evaluate_def] >>
       DEEP_INTRO_TAC some_intro >> rw [EXISTS_PROD] >>
       ntac 2 TOP_CASE_TAC >>
-      pairarg_tac >> gvs [] >>
-      qexists_tac ‘k’ >> rw [])
-  >- (rw [fbs_semantics_beh_def,
-          panSemTheory.evaluate_def] >>
-      rw [panPropsTheory.eval_upd_clock_eq] >>
-      DEEP_INTRO_TAC some_intro >> rw [] >>
-      FULL_CASE_TAC >> fs [])
+      pairarg_tac >> gvs [unclock_def])>>
+  rw [fbs_semantics_beh_def,
+      panSemTheory.evaluate_def] >>
+  rw [panPropsTheory.eval_upd_clock_eq] >>
+  DEEP_INTRO_TAC some_intro >> rw [] >>
+  FULL_CASE_TAC >> fs [unclock_def]
 QED
 
 Theorem itree_wbisim_neq:
@@ -546,7 +574,7 @@ Proof
 QED
 
 Theorem itree_semantics_beh_simps:
-  (itree_semantics_beh s Skip = SemTerminate (NONE, s with clock := 0) s.ffi.io_events) ∧
+  (itree_semantics_beh s Skip = SemTerminate (NONE, unclock s) s.ffi.io_events) ∧
   (eval s e = NONE ⇒
    itree_semantics_beh s (Dec v e prog) = SemFail)
 Proof
@@ -554,18 +582,18 @@ Proof
   >- (rw [itree_semantics_beh_def] >>
       DEEP_INTRO_TAC some_intro >> rw []
       >- (ntac 2 TOP_CASE_TAC >>
-          fs [panItreeSemTheory.h_prog_def,
+          fs [panItreeSemTheory.h_prog_def,unclock_def,
               panItreeSemTheory.mrec_sem_simps] >>
           fs [ltree_lift_cases] >>
           fs [Once itreeTauTheory.itree_wbisim_cases]) >>
       simp[EXISTS_PROD]>>
-      fs [panItreeSemTheory.h_prog_def,
+      fs [panItreeSemTheory.h_prog_def,unclock_def,
           panItreeSemTheory.mrec_sem_simps] >>
       fs [ltree_lift_cases] >>
       fs [Once itreeTauTheory.itree_wbisim_cases])>>
   rw [itree_semantics_beh_def]>>
   DEEP_INTRO_TAC some_intro >> rw [EXISTS_PROD]>>
-  fs [itree_semantics_beh_def,
+  fs [itree_semantics_beh_def,unclock_def,
       panItreeSemTheory.h_prog_def,
       panItreeSemTheory.h_prog_rule_dec_def] >>
   rpt CASE_TAC>>gvs[]>>
@@ -641,10 +669,10 @@ QED
 
 Theorem itree_sem_while_no_loop:
   eval s e = SOME (ValWord 0w) ⇒
-  itree_semantics_beh s (While e c) = SemTerminate (NONE,s) s.ffi.io_events
+  itree_semantics_beh s (While e c) = SemTerminate (NONE,unclock s) s.ffi.io_events
 Proof
   rw [itree_semantics_beh_def] >>
-  gvs [panItreeSemTheory.h_prog_def,
+  gvs [panItreeSemTheory.h_prog_def,unclock_def,
        panItreeSemTheory.h_prog_rule_while_def,
        Once itreeTauTheory.itree_iter_thm,
        panItreeSemTheory.mrec_sem_simps,
@@ -655,6 +683,224 @@ Proof
   ORELSE (qexists_tac ‘(SOME Error,s)’ >>
           rw [itreeTauTheory.itree_wbisim_refl])
 QED
+
+(** clock independence **)
+(* need newer HOL for this:
+Coinductive clk_indep:
+[~tau:]
+  (clk_indep (t:('a,'b) htree) t' ⇒ clk_indep (Tau t) (Tau t'))
+[~vis:]
+  ((case (e,e') of
+      (INL (r,s),INL (r,s')) => r = r' ∧ unclock s = unclock s'
+    | (INR (r,s),INR (r,s')) => r = r' ∧ unclock s = unclock s'
+    | _ => F) ∧
+   (∀a. clk_indep (g a) (g' a)) ⇒ clk_indep (Vis e g) (Vis e' g'))
+[~ret:]
+  (r=r' ∧ unclock s = unclock s' ⇒ clk_indep (Ret (r,s)) (Ret (rr,s)))
+End
+*)
+
+CoInductive clk_indep:
+  (clk_indep (t:('a,'b) htree) t' ⇒ clk_indep (Tau t) (Tau t')) ∧
+  ((case (e,e') of
+    | (INL (r,s),INL (r',s')) => r = r' ∧ unclock s = unclock s'
+    | (INR (r,f),INR (r',f')) => r = r' ∧
+                                 (∀a. unclock (SND (f a)) = unclock (SND (f' a)))
+    | _ => F) ∧
+   (∀a. clk_indep (g a) (g' a)) ⇒ clk_indep (Vis e g) (Vis e' g')) ∧
+  (r=r' ∧ unclock s = unclock s' ⇒ clk_indep (Ret (r,s)) (Ret (r',s')))
+End
+    
+Theorem h_prog_clock_shift:
+  ∀prog s k. mrec_sem (h_prog (prog,s)) = mrec_sem (h_prog (prog,s with clock := k))
+Proof
+
+Theorem h_prog_clock_clk_indep:
+  clk_indep (h_prog (prog,s)) (h_prog (prog,s with clock := k))
+Proof
+  irule clk_indep_coind>>
+  qexists_tac ‘λx y. ∃k. x = h_prog (prog, s) ∧
+                                y = h_prog (prog, s with clock := k)’>>
+  reverse $ rw[]>- metis_tac[]>>
+        
+  MAP_EVERY qid_spec_tac [‘k’,‘s’,‘prog’]>>
+  recInduct panItreeSemTheory.h_prog_ind>>
+  rw [panItreeSemTheory.h_prog_def,
+      panItreeSemTheory.h_prog_rule_dec_def,
+      panItreeSemTheory.h_prog_rule_assign_def,
+      panItreeSemTheory.h_prog_rule_store_def,
+      panItreeSemTheory.h_prog_rule_store_byte_def,
+      panItreeSemTheory.h_prog_rule_shmem_def,
+      panItreeSemTheory.h_prog_rule_seq_def,
+      panItreeSemTheory.h_prog_rule_cond_def,
+      panItreeSemTheory.h_prog_rule_raise_def,
+      panItreeSemTheory.h_prog_rule_return_def,
+      panItreeSemTheory.h_prog_rule_tick_def,
+      panItreeSemTheory.h_prog_rule_while_def,
+     panPropsTheory.eval_upd_clock_eq]>>
+  TRY (simp[unclock_def]>>NO_TAC)>>
+
+  CASE_TAC>>fs[]>>
+  pairarg_tac>>fs[]>>metis_tac[]
+
+simp[unclock_def]
+
+QED
+
+Theorem clock2:
+  ∀prog s. 
+  h_prog (prog, s) = Ret x ⇒
+  ∃y. h_prog (prog, s with clock := k + s.clock) = Ret y ∧
+      FST y = FST x ∧ unclock (SND y) = unclock (SND x)
+Proof
+  recInduct panItreeSemTheory.h_prog_ind>>
+  rw [panItreeSemTheory.h_prog_def,
+      panItreeSemTheory.h_prog_rule_dec_def,
+      panItreeSemTheory.h_prog_rule_assign_def,
+      panItreeSemTheory.h_prog_rule_store_def,
+      panItreeSemTheory.h_prog_rule_store_byte_def,
+(*      panItreeSemTheory.h_prog_rule_shmem_def,*)
+      panItreeSemTheory.h_prog_rule_call_def,
+      panItreeSemTheory.h_prog_rule_ext_call_def,
+      panItreeSemTheory.h_prog_rule_seq_def,
+      panItreeSemTheory.h_prog_rule_cond_def,
+      panItreeSemTheory.h_prog_rule_raise_def,
+      panItreeSemTheory.h_prog_rule_return_def,
+      panItreeSemTheory.h_prog_rule_tick_def,
+      panItreeSemTheory.h_prog_rule_while_def,
+      panPropsTheory.eval_upd_clock_eq]>>
+  TRY (fs[unclock_def]>>NO_TAC)>>fs[]>>
+  rpt (CASE_TAC>>fs[])>>
+
+  gvs[unclock_def,panSemTheory.empty_locals_def,panSemTheory.dec_clock_def]
+cheat (* tick *)
+cheat (* shmem *)
+(rpt (FULL_CASE_TAC>>fs[])>>gvs[]>>
+ fs[Once itreeTauTheory.itree_iter_thm,
+    panPropsTheory.eval_upd_clock_eq]>>
+ rpt (CASE_TAC>>gvs[unclock_def]))>-
+   (rpt (FULL_CASE_TAC>>fs[])>>gvs[unclock_def]>>
+    fs[panPropsTheory.eval_upd_clock_eq]>>
+    fs[panSemTheory.lookup_code_def,option_case_eq]>>
+    FULL_CASE_TAC>>gvs[])>>
+  rpt (CASE_TAC>>fs[])>>gvs[unclock_def]
+QED
+
+Theorem clock1:
+  mrec_sem (h_prog (prog, s)) = Ret x ⇒
+  ∃y. mrec_sem (h_prog (prog, s with clock := k + s.clock)) = Ret y ∧
+      FST y = FST x ∧ unclock (SND y) = unclock (SND x)
+Proof
+  strip_tac>>
+  fs[panItreeSemTheory.mrec_sem_def]>>
+  Cases_on ‘h_prog (prog,s)’>>fs[]>-
+   (imp_res_tac clock2>>
+    first_x_assum $ qspec_then ‘k’ assume_tac>>
+    fs[]>>
+    gvs[Once itreeTauTheory.itree_iter_thm]>>
+    gvs[Once itreeTauTheory.itree_iter_thm])>-
+   gvs[Once itreeTauTheory.itree_iter_thm]>>
+  Cases_on ‘a’>>
+  gvs[Once itreeTauTheory.itree_iter_thm]>>
+  pairarg_tac>>fs[]
+QED
+
+
+Theorem clock0:
+  ltree_lift query_oracle s.ffi (mrec_sem (h_prog (prog,s))) = Ret (r,s') ⇒
+  ∀k. ∃r' s''. ltree_lift query_oracle s.ffi (mrec_sem (h_prog (prog,s with clock := s.clock + k))) = Ret (r',s'') ∧ r' = r ∧ unclock s' = unclock s''
+Proof
+  strip_tac>>
+  strip_tac>>
+  fs[ltree_lift_def]>>
+  Cases_on ‘mrec_sem (h_prog (prog,s))’>>fs[]>-
+   (imp_res_tac clock1>>
+    first_x_assum $ qspec_then ‘k’ assume_tac>>
+    fs[]>>
+    gvs[Once itreeTauTheory.itree_iter_thm]>>
+    gvs[Once itreeTauTheory.itree_iter_thm]>>
+    Cases_on ‘y’>>gvs[])>-
+   gvs[Once itreeTauTheory.itree_iter_thm]>>
+  Cases_on ‘a’>>
+  gvs[Once itreeTauTheory.itree_iter_thm]>>
+  pairarg_tac>>fs[]
+QED
+
+
+Theorem itree_beh_clock_shift:
+  itree_semantics_beh s prog = itree_semantics_beh (s with clock := k) prog
+Proof
+  simp[itree_semantics_beh_def]>>
+  DEEP_INTRO_TAC some_intro >> rw [] >>
+  DEEP_INTRO_TAC some_intro >> rw [] >-
+
+   (ntac 2 (CASE_TAC>>fs[])>>
+    TRY (ntac 2 (CASE_TAC>>fs[]))>>
+    imp_res_tac clock0>>
+    first_x_assum $ qspec_then ‘k’ assume_tac>>fs[]>>
+    drule itreeTauTheory.itree_wbisim_sym>>strip_tac>>
+    drule itreeTauTheory.itree_wbisim_trans>>
+    disch_then $ rev_drule_at Any>>
+    simp[Once itreeTauTheory.itree_wbisim_cases]>>
+    gvs[FORALL_PROD,ltree_lift_cases,unclock_def])>>
+
+
+
+  fs[LAMBDA_PROD,FORALL_PROD]
+        
+  
+  recInduct panItreeSemTheory.h_prog_ind>>
+  rw [panItreeSemTheory.h_prog_def,
+      panItreeSemTheory.h_prog_rule_dec_def,
+      panItreeSemTheory.h_prog_rule_assign_def,
+      panItreeSemTheory.h_prog_rule_store_def,
+      panItreeSemTheory.h_prog_rule_store_byte_def,
+      panItreeSemTheory.h_prog_rule_shmem_def,
+      panItreeSemTheory.h_prog_rule_seq_def,
+      panItreeSemTheory.h_prog_rule_cond_def,
+      panItreeSemTheory.h_prog_rule_raise_def,
+      panItreeSemTheory.h_prog_rule_return_def,
+      panItreeSemTheory.h_prog_rule_tick_def,
+      panItreeSemTheory.h_prog_rule_while_def]>>
+  simp[Once itreeTauTheory.itree_iter_thm,
+       panItreeSemTheory.mrec_sem_simps,
+       panPropsTheory.eval_upd_clock_eq,
+       ltree_lift_cases] >>
+(*  fs [Once itreeTauTheory.itree_wbisim_cases]>>*)
+  TRY
+  (DEEP_INTRO_TAC some_intro >> rw [] >>
+  DEEP_INTRO_TAC some_intro >> rw [] >>
+  rpt CASE_TAC>>fs[unclock_def,FORALL_PROD]>>
+  fs [Once itreeTauTheory.itree_wbisim_cases]>>NO_TAC)
+
+
+  (* dec *)
+  CASE_TAC>>fs[]>>
+  DEEP_INTRO_TAC some_intro >> rw [] >>
+  DEEP_INTRO_TAC some_intro >> rw [] >>
+  rpt (CASE_TAC>>fs[])>>
+  fs [panItreeSemTheory.mrec_sem_simps,ltree_lift_cases,
+      Once itreeTauTheory.itree_wbisim_cases,
+      Once itreeTauTheory.strip_tau_cases,
+      unclock_def,FORALL_PROD]>>
+
+
+
+  rpt CASE_TAC>>fs[unclock_def,FORALL_PROD]>>
+
+
+
+
+  gvs [panItreeSemTheory.h_prog_def,unclock_def,
+       panItreeSemTheory.h_prog_rule_while_def,
+       Once itreeTauTheory.itree_iter_thm,
+       panItreeSemTheory.mrec_sem_simps,
+       ltree_lift_cases] >>
+
+  
+QED
+
+(** end : clock **)
 
 (* TODO: Need to prove the correspondence for While more directly
  to better understand what is required here... *)
@@ -683,8 +929,7 @@ Proof
                   (* THIS IS VERY STRANGE... the states are messed up. *)
                   cheat) >>
               cheat)
-          >- (CONV_TAC SYM_CONV >>
-              rw [itree_sem_while_no_loop])
+          >- fs[itree_sem_while_no_loop,unclock_def]
           >- (rw [itree_sem_while_fails])
           >- (rw [itree_sem_while_fails])) >>
       (* All remaining terms... for convg case *)
